dataplane/Examples/Batch_op.thy
@@ -3,30 +3,36 @@ theory Batch_op
 imports
   Dataplane.Timely_Stream
   Dataplane.Timely_Infrastructure
+  "../MyProduct_Instances"
 begin
 
 term "show_list show_nat"
 
-term trace
+abbreviation "show_myprod \<equiv> (\<lambda> s1 s2. show_prod s1 s2 o to_prod)"
 
 definition batch_op where
   "batch_op ips ops comb os logic = notifier_op ips ops os 
    (\<lambda> os compl_caps.
     let comb_caps = comb compl_caps in
     let compl_batches = (\<lambda> p t. map (de1 os o fst) (filter (\<lambda> (d, t'). t' = t \<and> t \<in> set (comb_caps p)) (input os p))) in
+    let sorted_ts = (\<lambda> p. map from_prod (sort (map to_prod (rmdups {} (map snd (filter (\<lambda> (d, t). t \<in> set (comb_caps p)) (input os p))))))) in
+    let ts = (\<lambda> p. rmdups {} (map snd (filter (\<lambda> (d, t). t \<in> set (comb_caps p)) (input os p)))) in
     let os = os\<lparr> input := (\<lambda> p. filter (\<lambda> (d, t). t \<notin> set (comb_caps p)) (input os p)) \<rparr> in
-    let outs_drops = logic compl_batches comb_caps in
+    let outs_drops = logic compl_batches ts comb_caps in
     cimage (\<lambda> (outs, drops). drop_caps (produces os (map (\<lambda> (d, cap). (en2 os d, cap)) outs)) drops) outs_drops)"
+
 
 definition batch_fun_op where
   "batch_fun_op os f = batch_op {|(1 :: 1)|} {|(1 :: 1)|} id os
-   (\<lambda> compl_batches caps. {| (concat (map (\<lambda> t. map (\<lambda> x. (x, Cap t 1)) (f (compl_batches 1 t))) (rmdups {} (caps 1))), map (\<lambda> t. Cap t 1) (caps 1)) |})"
+   (\<lambda> compl_batches ts caps. {| (concat (map (\<lambda> t. map (\<lambda> x. (x, Cap t 1)) (f (compl_batches 1 t))) (ts 1)), map (\<lambda> t. Cap t 1) (caps 1)) |})"
 
+
+(*
 definition diff_op where
   "diff_op os = batch_op {|(1 :: 2), 2|} {|1|} 
    (\<lambda> compl_caps p. if p = 1 then filter (\<lambda> t. t \<in> set (compl_caps 2)) (compl_caps 1) else filter (\<lambda> t. t \<in> set (compl_caps 1)) (compl_caps 2))
    (os\<lparr> de1 := projl, en2 := Inr \<rparr>)
-   (\<lambda> compl_batches caps. 
+   (\<lambda> compl_batches ts caps. 
    {| (map (\<lambda> t. (mset (compl_batches 1 t) - mset (compl_batches 2 t), Cap t 1)) (rmdups {} (caps 1)),
        map (\<lambda> t. Cap t 1) (caps 1) @ map (\<lambda> t. Cap t 2) (caps 2)) |})"
 
@@ -39,5 +45,5 @@ definition batch_ty2_op where
     let outs_drops = logic compl_batches comb_caps in
     cimage (\<lambda> (outs, drops). drop_caps (produces os (map (\<lambda> (d, cap). (en2 os d, cap)) outs)) drops) outs_drops)"
 
-
+ *)
 end
